theories/Temporal.v
@@ -1,6 +1,6 @@
 From Coq Require Import Lists.List.
-From Mecha Require Import RealResource REnvironment Term Functional Resource Cell Typing VContext Typ
-               Resources Evaluation RContext.
+From Mecha Require Import RFlows REnvironment Term Functional Resource Cell Typing VContext Typ
+               Resources Evaluation RContext RFlow.
 
 (** * Transition - Temporal
 
@@ -16,83 +16,63 @@ Reserved Notation "'Wfₜₜ(' Re , Rf )" (at level 50).
 
 (** *** Definition *)
 
-Inductive temporal : RealResources.t -> RealResources.t -> Λ -> Λ -> Prop :=
- TT_instant : forall Vin Vout _tv (R R' : RealResources.t) (P P' : Λ),
+Inductive temporal : 𝐅 -> 𝐅 -> Λ -> Λ -> Prop :=
+  | TT_instant : forall Vin Vout _tv (R R' : 𝐅) (P P' : Λ),
 
-                    (Vin = RE.embeds (RealResources.nexts R))%re ->
+                    (Vin = RFlows.nexts R)%re ->
                     ⪡ Vin ; unit ; P ⪢ ⭆ ⪡ Vout ; _tv ; P' ⪢ ->
-                    R' = RealResources.puts (RE.extracts Vout) R -> 
+                    (R' = RFlows.puts Vout R) -> 
                     
-                    temporal R R' P P'.
+                    temporal R R' P P'
+  | TT_trans : forall R R' R'' (P P' P'' : Λ), 
+                  temporal R R' P P' -> 
+                  temporal R' R'' P' P'' -> 
+                  temporal R R'' P P''.
 
 Notation "'⟦' R ';' P '⟧' '⟾' '⟦' R1 ';' P1 '⟧'" := (temporal R R1 P P1) 
                                                      (at level 30, R constr, R1 constr,
                                                          P custom rsf, P1 custom rsf, 
                                                         no associativity).
 
-Inductive multi_temporal : RealResources.t -> RealResources.t -> Λ -> Λ -> Prop :=
-  TT_step : forall R R' R'' (P P' P'' : Λ), 
-                  ⟦ R ; P ⟧ ⟾ ⟦ R' ; P' ⟧ -> 
-                  multi_temporal R' R'' P' P'' -> 
-                  multi_temporal R R'' P P''.
+Inductive wf_env_TT : ℜ -> 𝐅 -> Prop :=
+  | wfTT_empty  : forall (Re : ℜ) (Fl : 𝐅), 
+                     isEmptyᵣᵪ(Re) -> 
+                     isEmptyᵣₔ(Fl) -> Wfₜₜ(Re,Fl)
 
-Notation "'⟦' R ';' P '⟧' '⟾⋆' '⟦' R1 ';' P1 '⟧'" := (multi_temporal R R1 P P1) 
-                                                     (at level 30, R constr, R1 constr,
-                                                         P custom rsf, P1 custom rsf, 
-                                                        no associativity).
-
-Inductive wf_env_TT : ℜ -> RealResources.t -> Prop :=
-  | wfTT_empty  : forall (Re : ℜ) (Fl : RealResources.t), 
-                     isEmptyᵣᵪ(Re) -> Wfₜₜ(Re,nil)
-
-  | wfTT_init   : forall (Re Re' : ℜ) (Fl : RealResources.t) (τ τ' : Τ) (r : RealResource.t),
+  | wfTT_add   : forall (Re Re' : ℜ) (Fl Fl' : 𝐅) (τ τ' : Τ) (r : RFlow.t),
       Wfₜₜ(Re,Fl) ->
       Addᵣᵪ (newᵣᵪ(Re)) (τ,τ') Re Re' ->
+      Addᵣₔ (newᵣₔ(Fl)) r Fl Fl' ->
       Streams.ForAll (fun v => ∅ᵥᵪ ⋅ Re ⊫ {Streams.hd v} ∈ τ') (fst r) -> 
       Streams.ForAll (fun v => ∅ᵥᵪ ⋅ Re ⊫ {Streams.hd v} ∈ τ) (snd r) -> 
-      Wfₜₜ(Re',Fl ++ (r :: nil))
+      Wfₜₜ(Re',Fl')
 
   | wfTT_update : forall (Re : ℜ) (V : 𝓥) Rf,
                     Wfᵣₜ(Re,V) -> 
                     Wfₜₜ(Re,Rf) ->
-                    Wfₜₜ(Re,RealResources.puts (RE.extracts V) Rf)
+                    Wfₜₜ(Re,RFlows.puts V Rf)
 where "'Wfₜₜ(' Re , Fl )" := (wf_env_TT Re Fl).
 
 Lemma wf_env_TT_to_fT Re Fl : 
-  Wfₜₜ(Re,Fl) -> Wfᵣₜ(Re,RE.embeds (RealResources.nexts Fl)).
-Proof.
-  intro inst; induction inst; simpl.
-  - unfold RE.embeds; simpl; apply wfFT_empty; auto.
-    apply RE.OP.P.empty_1.
-  - destruct r; simpl in *. unfold RealResources.nexts.
-    rewrite map_app; simpl. unfold RE.embeds.
-    unfold RE.embeds_gen; rewrite <- fold_left_rev_right. 
-    fold RE.embeds_func_revert. rewrite rev_unit; simpl.
-    rewrite fold_left_rev_right. unfold RE.embeds_func_revert.
-    replace (fold_left (fun (x : RE.t) (y : Λ) => RE.embeds_func x y) (map RealResource.next Fl) (∅ᵣᵦ))
-    with (RE.embeds (RealResources.nexts Fl)); auto.
-    unfold RE.embeds_func.
-    
-    destruct s; simpl in *. inversion H0; simpl in *.
-    eapply wfFT_init with (v := λ); eauto.
-    unfold RE.OP.P.Add; reflexivity.
-  - admit.
+  Wfₜₜ(Re,Fl) -> Wfᵣₜ(Re,RFlows.nexts Fl).
+Proof. 
+  intros. induction H.
+  - apply wfFT_empty; auto. rewrite RFlows.nexts_Empty; auto.
+    apply RFlows.OP.P.empty_1.
+  - apply (wfFT_add Re Re' (RFlows.nexts Fl) (RFlows.nexts Fl')
+                     τ τ' (RFlow.next r)); auto.
+    -- unfold RE.OP.P.Add. apply RFlows.nexts_Add_spec; auto; admit.
+    -- destruct r; simpl in *; apply H2.
+  - 
 Admitted.
 
 (** *** Initialization *)
-
-Theorem initialization_unused : forall l,
-  RE.For_all (fun _ v => Cell.unused v) (RE.embeds l).
-Proof.
-  intros. apply RE.embedding_Forall_unused.
-  unfold RE.For_all; intros. inversion H.
-Qed.
 
 Lemma resource_used_init_unused : forall Re t α β R l V,
   ∅ᵥᵪ ⋅ Re ⊫ t ∈ (α ⟿ β ∣ R) ->
   halts t ->
   Wfᵣₜ(Re,V) ->
-  (V = (RE.embeds l))%re ->
+  (V = (RFlows.nexts l))%re ->
   
   (forall r, (r ∈ R)%rs -> RE.unused r V).
 Proof.
@@ -101,15 +81,21 @@ Proof.
   apply typing_Re_R with (r := r) in H; auto.
   apply wf_env_fT_in with (V := V) in H; auto.
   rewrite H2 in *. destruct H; apply RE.OP.P.find_1 in H.
-  apply initialization_unused in H as H'; destruct x; inversion H'.
-  exists λ. now rewrite H2.
+  assert (r ∈ᵣₔ l). { rewrite RFlows.nexts_in_iff. exists x. now apply RE.OP.P.find_2. }
+  apply RFlows.nexts_unused in H0. destruct H0. rewrite <- H2 in H0.
+  now exists x0.
 Qed. 
+
+Section safety.
+
+Hypothesis all_arrow_halting : forall Re t α β,
+  ∅ᵥᵪ ⋅ Re ⊫ arr(t) ∈ (α ⟿ β ∣ ∅ᵣₛ) -> forall v, ∅ᵥᵪ ⋅ Re ⊫ v ∈ α -> halts <[t v]>.
 
 
 (** *** Proof of typing preservation through the temporal transition *)
 Theorem temporal_preserves_typing (Re : ℜ) Rf Rf' (P P' : Λ) (R : resources) :
 
-    (* (1) *) halts P -> (* (2) *) RealResources.halts Rf -> (* (3) *) all_arrow_halting ->
+    (* (1) *) halts P -> (* (2) *) RFlows.halts Rf ->
 
     (* (1) *) ∅ᵥᵪ ⋅ Re ⊫ P ∈ (𝟙 ⟿ 𝟙 ∣ R) ->
     (* (3) *) ⟦ Rf ; P ⟧ ⟾ ⟦ Rf' ; P' ⟧ ->
@@ -117,69 +103,72 @@ Theorem temporal_preserves_typing (Re : ℜ) Rf Rf' (P P' : Λ) (R : resources) 
 
   (*----------------------------------------------------*)
       ∅ᵥᵪ ⋅ Re ⊫ P' ∈ (𝟙 ⟿ 𝟙 ∣ R) /\ Wfₜₜ(Re,Rf') /\ 
-       (* (7) *) halts P' /\ (* (8) *) RealResources.halts Rf'.
+       (* (7) *) halts P' /\ (* (8) *) RFlows.halts Rf'.
 Proof.
-  intros HltP HltRf HlAll HwP HTT Hinst; inversion HTT; subst.
-  apply wf_env_TT_to_fT in Hinst as Hinst'.
-  eapply functional_preserves_typing in H0; eauto.
-  - repeat split; destruct H0 as [_ [_ [HinstV [_ [_ [HwP' [HltP' [_ HltVout]]]]]]]]; auto.
-    -- constructor; auto.
-    -- apply RealResources.halts_puts; auto. now apply RE.halts_extract.
-  - exists <[unit]>; split; auto.
-  - apply REnvironment.halts_nexts in HltRf. unfold RE.halts; intros. rewrite H in *.
-    eapply HltRf; eauto. 
-  - now rewrite H.
-Qed.
-
-(** *** Proof of typing preservation through multi temporal transitions *)
-Theorem multi_temporal_preserves_typing (Re : ℜ) Rf Rf' (P P' : Λ) (R : resources) :
-    (* (1) *) halts P -> (* (2) *) RealResources.halts Rf -> (* (3) *) all_arrow_halting ->
-
-    (* (1) *) ∅ᵥᵪ ⋅ Re ⊫ P ∈ (𝟙 ⟿ 𝟙 ∣ R) ->
-    (* (3) *) ⟦ Rf ; P ⟧ ⟾⋆ ⟦ Rf' ; P' ⟧ ->
-              Wfₜₜ(Re,Rf) ->
-
-  (*----------------------------------------------------*)
-      ∅ᵥᵪ ⋅ Re ⊫ P' ∈ (𝟙 ⟿ 𝟙 ∣ R) /\ Wfₜₜ(Re,Rf') /\ 
-       (* (7) *) halts P' /\ (* (8) *) RealResources.halts Rf'.
-Proof.
-  intros HltP HltRf HAll HwP HTT; induction HTT; subst; intros.
-  eapply temporal_preserves_typing in H as [HwP' [HWf [HltP' HlR0]]]; eauto.
-Qed.
+  intros HltP HltRf HwP HTT; revert Re R HltP HltRf HwP. 
+  induction HTT; subst; intros Re R1 HlP HlRf HwP Hwf.
+  - apply wf_env_TT_to_fT in Hwf as Hwf'.
+    eapply functional_preserves_typing in H0; eauto.
+    -- destruct H0 as [_ [_ [HwfV [_ [_ [HwP' [HltP' [_ HltVout]]]]]]]].
+       split; auto; split.
+       + eapply wfTT_update; auto.
+       + split; auto. apply RFlows.halts_puts; auto.
+    -- exists <[unit]>; split; auto.
+    -- apply RFlows.halts_nexts in HlRf. eapply RE.halts_eq; eauto.
+    -- now rewrite H.
+  - apply IHHTT1 in HwP as IH; auto. destruct IH as [HwP' [Hwf' [HlP' HlR']]].
+    apply IHHTT2; assumption.
+Qed. 
 
 
-Theorem progress_of_temporal (Re : ℜ) (Rf : RealResources.t) (P : Λ) (R : resources) :
+Theorem progress_of_temporal (Re : ℜ) (Rf : 𝐅) (P : Λ) (R : resources) :
 
-  (* (1) *) halts P -> (* (2) *) RealResources.halts Rf -> (* (3) *) all_arrow_halting ->
+  (* (1) *) halts P -> (* (2) *) RFlows.halts Rf ->
 
   (* (4) *) ∅ᵥᵪ ⋅ Re ⊫ P ∈ (𝟙 ⟿ 𝟙 ∣ R) -> (* (5) *) Wfₜₜ(Re,Rf) ->
   
   (*-------------------------------------------------------------------------------------------------*)
     exists Rf' P',  (* (6) *) ⟦ Rf ; P ⟧ ⟾ ⟦ Rf' ; P' ⟧ /\ 
-                    (* (7) *) halts P' /\ (* (8) *) RealResources.halts Rf'.
+                    (* (7) *) halts P' /\ (* (8) *) RFlows.halts Rf'.
 Proof.
-  intros HltP HltRf HlAll HwP Hinst. 
+  intros HltP HltRf HwP Hinst. 
   assert (HwU : ∅ᵥᵪ ⋅ Re ⊫ unit ∈ 𝟙). { now constructor. }
-  remember (RE.embeds (RealResources.nexts Rf)) as Vin.
+  remember (RFlows.nexts Rf) as Vin.
 
   eapply progress_of_functional with (V := Vin) in HwU; eauto.
   - destruct HwU as [Vout [tv' [P' [HfT [HltP' [Hltv' HltVout]]]]]].
-    exists (RealResources.puts (RE.extracts Vout) Rf); exists P'; repeat split; auto.
+    exists (RFlows.puts Vout Rf); exists P'; split.
     -- econstructor; eauto; subst; reflexivity.
-    -- apply RealResources.halts_puts; auto. now apply RE.halts_extract.
+    -- split; auto. apply RFlows.halts_puts; auto.
   - exists <[unit]>; split; auto.
-  - apply REnvironment.halts_nexts in HltRf. unfold RE.halts; intros. rewrite HeqVin in *.
-    eapply HltRf; eauto. 
+  - apply RFlows.halts_nexts in HltRf; now subst.
   - subst. now apply wf_env_TT_to_fT.
   - apply wf_env_TT_to_fT in Hinst.
     destruct HltP as [P' [HmeT HltP']].
     eapply multi_preserves_typing in HwP; eauto.
     intros. apply typing_Re_R with (r := r) in HwP; auto.
-    rewrite wf_env_fT_in in HwP; eauto.
-    unfold RE.unused. 
-    assert (RE.For_all (fun _ v => Cell.unused v) (RE.embeds (RealResources.nexts Rf))).
-    { apply initialization_unused. }
-    unfold RE.For_all in *. destruct HwP. apply RE.OP.P.find_1 in H1.
-    apply H0 in H1 as Hunsd. destruct x; inversion Hunsd. exists λ.
-    now rewrite HeqVin.
+    rewrite wf_env_fT_in in HwP; eauto; subst.
+    apply RFlows.nexts_unused. now rewrite RFlows.nexts_in_iff.
 Qed.
+
+(*
+(** *** Proof of Resource safety *)
+Theorem safety_resources_interaction (Re : ℜ) (Rf : 𝐅) (t : Λ) (τ τ' : Τ) (R : resources) :
+
+    (* (1) *) halts t -> (* (2) *) RFlows.halts Rf ->
+
+    (* (3) *) Wfₜₜ(Re,Rf) -> (* (4) *) ∅ᵥᵪ ⋅ Re ⊫ t ∈ (τ ⟿ τ' ∣ R) ->
+
+  (*-----------------------------------------------------------------------------------------------*)
+    forall (tv : Λ), (* (5) *) halts tv -> (* (6) *) ∅ᵥᵪ ⋅ Re ⊫ tv ∈ τ -> 
+
+    exists (V' : 𝓥) (tv' t' : Λ), 
+      (* (7) *) ⪡ V ; tv ; t ⪢ ⭆ ⪡ V' ; tv' ; t' ⪢ /\
+
+      (* (8) *) (forall (r : resource), (r ∉ R)%rs /\ (r ∈ᵣᵦ V) -> V ⌊r⌋ᵣᵦ = V' ⌊r⌋ᵣᵦ) /\
+      (* (9) *) (forall (r : resource), (r ∈ R)%rs -> RE.used r V').
+Proof.
+Admitted.
+*)
+
+End safety.
