theories/Environments_Contexts/RFlows.v
@@ -1,0 +1,372 @@
+From Mecha Require Import Term Evaluation Resource REnvironment Cell RFlow.
+From DeBrLevel Require Import MapExtInterface MapExt.
+From MMaps Require Import MMaps.
+
+Module RFlows <: EqualityType.
+
+Module Raw := MMaps.OrdList.Make Resource.
+Module Ext := MapETLVL RFlow Raw.
+
+Include Ext.
+Import Raw OP.P.
+
+Definition nexts_func x v V := ⌈x ⤆ (Cell.inp (RFlow.next v))⌉ᵣᵦ V.
+
+Definition nexts (fl : RFlows.t) : REnvironment.t := 
+  fold nexts_func fl (∅ᵣᵦ).
+
+Definition puts_func V x v fl := 
+  match V⌊x⌋ᵣᵦ with 
+    | Some (⩽ … v' ⩾) =>  add x (RFlow.put v' v) fl
+    |  _ => fl 
+  end.
+
+Definition puts (Vout : REnvironment.t) (fl : RFlows.t) : RFlows.t :=
+  fold (puts_func Vout) fl empty.
+
+Definition halts (fl : RFlows.t) := forall (r : resource) v, 
+ find r fl = Some v -> RFlow.halts v.
+
+
+
+Hint Resolve REnvironment.eq_equiv : core.
+
+(** *** Nexts *)
+
+#[export]
+Instance nexts_prop : 
+  Proper (Logic.eq ==> Logic.eq ==> REnvironment.eq ==> REnvironment.eq) nexts_func.
+Proof.
+  repeat red; intros; subst. unfold nexts_func; now rewrite H1.
+Qed.
+
+Lemma nexts_diamond : Diamond REnvironment.eq nexts_func.
+ repeat red; intros. rewrite <- H0. rewrite <- H1.
+ unfold nexts_func. rewrite REnvironment.OP.P.add_add_2; auto.
+Qed.
+
+Hint Resolve nexts_prop nexts_diamond : core.
+
+Lemma nexts_Empty t : Empty t -> ((nexts t) = ∅ᵣᵦ)%re.
+Proof. 
+  intros; unfold nexts. rewrite fold_Empty; auto. reflexivity. 
+Qed.
+
+Lemma nexts_Add_spec x v t t' : 
+  ~ In x t ->
+  Add x v t t' -> ((nexts t') = ⌈x ⤆ (Cell.inp (RFlow.next v))⌉ᵣᵦ (nexts t))%re.
+Proof.
+  intros. unfold nexts. 
+  apply fold_Add with (A := REnvironment.t) (eqA := REnvironment.eq) 
+                      (f := nexts_func) (i := ∅ᵣᵦ) in H0; auto.
+Qed.
+
+#[export]
+Instance nexts_eq : Proper (eq ==> REnvironment.eq) nexts.
+Proof.
+  repeat red; intros; revert y0 y H. induction x using map_induction; intros.
+  - assert (Empty y). { now rewrite H0 in *. }
+    rewrite nexts_Empty; auto. rewrite nexts_Empty; auto.
+  - destruct (In_dec y x3).
+    -- destruct i; apply find_1 in H2. rewrite <- add_id in H2.
+       rewrite <- add_remove_1 in H2. assert (~ In x3 (remove x3 y)).
+       { intro. rewrite remove_in_iff in H3. destruct H3. now apply H3. }
+       rewrite <- H2 in H1. assert (x = e).
+       { 
+        apply mapsto_fun with (x := x3) (m := x2). 
+        - rewrite H1. apply add_mapsto_new; auto.
+        - unfold Add in H0. rewrite H0. apply add_mapsto_new; auto.
+       }
+       subst. assert (Add x3 e (remove x3 y) y).
+       { unfold Add. now rewrite H2. }
+       rewrite (nexts_Add_spec x3 e x1 x2); auto.
+       rewrite (nexts_Add_spec x3 e (remove x3 y) y); auto.
+       destruct (Resource.eq_dec x3 y0); subst.
+       + repeat rewrite REnvironment.OP.P.add_eq_o; auto.
+       + repeat rewrite REnvironment.OP.P.add_neq_o; auto.
+         apply IHx1.
+         unfold eq. unfold eq in H1. rewrite Equal_mapsto_iff in *; intros.
+         destruct (Resource.eq_dec k x3); subst.
+         ++ split; intros.
+            * exfalso. apply H. now exists e0.
+            * exfalso; apply H3. now exists e0.
+         ++ split; intros.
+            * rewrite <- add_neq_mapsto_iff; eauto.
+              rewrite <- H1. unfold Add in H0. rewrite H0.
+              rewrite add_neq_mapsto_iff; auto.
+            * rewrite <- add_neq_mapsto_iff; eauto.
+              unfold Add in H0. rewrite <- H0. rewrite H1.
+              rewrite add_neq_mapsto_iff; auto.
+    -- assert (Add x3 e x1 y). { unfold Add in *; rewrite <- H1; assumption. }
+       rewrite (nexts_Add_spec x3 e x1 x2); auto.
+       rewrite (nexts_Add_spec x3 e x1 y); auto. 
+Qed.
+
+Lemma nexts_in_iff r fl : In r fl <-> r ∈ᵣᵦ (nexts fl).
+Proof.
+  revert r; induction fl using map_induction; split; intros.
+  - exfalso. destruct H0. now apply (H r x).
+  - rewrite nexts_Empty in H0; auto. inversion H0; inversion H1.
+  - destruct (Resource.eq_dec x r); subst.
+    -- rewrite nexts_Add_spec; eauto. 
+       rewrite REnvironment.OP.P.add_in_iff; now left.
+    -- rewrite nexts_Add_spec; eauto.
+       rewrite REnvironment.OP.P.add_in_iff; right.
+       unfold Add in *. rewrite H0 in *.
+       rewrite add_in_iff in H1; destruct H1; try (contradiction).
+       now rewrite <- IHfl1.
+  - destruct (Resource.eq_dec x r); subst.
+    -- unfold Add in *; rewrite H0. rewrite add_in_iff; now left.
+    -- rewrite nexts_Add_spec in *; eauto.
+       unfold Add in *. rewrite H0 in *.
+       rewrite add_in_iff; right. 
+       rewrite REnvironment.OP.P.add_in_iff in H1; 
+       destruct H1; try (contradiction).
+       now rewrite IHfl1.
+Qed. 
+
+Lemma nexts_unused r fl : In r fl -> REnvironment.unused r (nexts fl).
+Proof.
+  revert r; induction fl using map_induction; unfold REnvironment.unused; intros.
+  - exfalso. destruct H0. now apply (H r x).
+  - destruct H1. apply find_1 in H1. rewrite H0 in *.
+    destruct (Resource.eq_dec r x); subst.
+    -- rewrite add_eq_o in H1; auto. inversion H1; subst; clear H1.
+       exists (RFlow.next x0); rewrite nexts_Add_spec; eauto.
+       rewrite REnvironment.OP.P.add_eq_o; auto.
+    -- assert (In r fl1). 
+       { rewrite add_neq_o in H1; auto. exists x0. now apply find_2. }
+       apply IHfl1 in H2; destruct H2. exists x1.
+       rewrite nexts_Add_spec; eauto.
+       rewrite REnvironment.OP.P.add_neq_o; auto.
+Qed.   
+
+(** *** Puts *)
+
+#[export]
+Instance puts_prop V :
+  Proper (Logic.eq ==> Logic.eq ==> eq ==> eq) (puts_func V).
+Proof.
+  repeat red; intros; subst; unfold puts_func. destruct (V⌊y⌋ᵣᵦ); auto.
+  destruct r; auto. now rewrite H1.
+Qed.
+
+Lemma puts_diamond V : Diamond Equal (puts_func V).
+Proof. 
+  repeat red; intros; unfold puts_func. 
+  destruct (V⌊k⌋ᵣᵦ) eqn:HfV; destruct (V⌊k'⌋ᵣᵦ) eqn:HfV'.
+  -- destruct r,r0; try 
+     (rewrite <- H1; rewrite <- H0; unfold puts_func;
+      now rewrite HfV', HfV).
+     rewrite <- H1; rewrite <- H0; unfold puts_func.
+     rewrite HfV',HfV. rewrite add_add_2; auto.
+  -- destruct r; try 
+     (rewrite <- H1; rewrite <- H0; unfold puts_func;
+      now rewrite HfV', HfV).
+  -- destruct r; try 
+     (rewrite <- H1; rewrite <- H0; unfold puts_func;
+      now rewrite HfV', HfV).
+  -- rewrite <- H1; rewrite <- H0; unfold puts_func.
+     now rewrite HfV', HfV.
+Qed.
+
+Hint Resolve puts_prop puts_diamond : core.
+
+Lemma puts_Empty V fl : Empty fl -> eq (puts V fl) empty.
+Proof.
+  intros; unfold puts,eq. rewrite fold_Empty; auto; reflexivity.
+Qed.
+
+Lemma puts_Add_spec r v V fl fl' : 
+  ~ In r fl -> Add r v fl fl' -> eq (puts V fl') ((puts_func V) r v (puts V fl)).
+Proof.
+  intros. unfold puts, eq. now rewrite fold_Add; eauto.
+Qed.
+
+
+(** *** Halts *)
+
+#[export]
+Instance halts_eq : Proper (eq ==> iff) halts.
+Proof.
+  repeat red; intros; split; intros.
+  - unfold eq,halts in *; intros. rewrite <- H in *.
+    eapply H0; eauto.
+  - unfold eq,halts in *; intros. rewrite H in *.
+    eapply H0; eauto.
+Qed.
+
+Lemma halts_add_spec : forall m x v,
+  (RFlow.halts v) /\ halts m -> halts (add x v m).
+Proof.
+  intros m x v. intros [Hltv Hltm]; unfold halts; intros r v' Hfi.
+  rewrite OP.P.add_o in Hfi; destruct (Resource.eq_dec x r); subst; inversion Hfi; subst; auto.
+  apply Hltm in Hfi; auto.
+Qed.
+
+Lemma halts_add_spec_1 : forall m x v,
+  ~ In x m -> halts (add x v m) -> (RFlow.halts v) /\ halts m.
+Proof.
+  intros; split.
+  - unfold halts in *. apply (H0 x v). now rewrite add_eq_o.
+  - unfold halts in *. intros r v' HfV. destruct (Resource.eq_dec x r).
+    -- subst. exfalso. apply H. exists v'; now apply find_2.
+    -- apply (H0 r). rewrite add_neq_o; auto.
+Qed.
+
+Lemma halts_nexts t : 
+  halts t -> REnvironment.halts (nexts t).
+Proof.
+  induction t using map_induction; intros Hlt0; unfold REnvironment.halts; intros.
+  - unfold nexts in *. rewrite fold_Empty in H0; auto.
+   inversion H0.
+  - rewrite nexts_Add_spec in H1; eauto. 
+    unfold Add in H0; rewrite H0 in *. 
+    apply halts_add_spec_1 in Hlt0 as [Hle Hlt1]; auto.
+    apply IHt1 in Hlt1 as IH; clear IHt1.
+    destruct (Resource.eq_dec x r); subst.
+    -- rewrite REnvironment.OP.P.add_eq_o in H1; auto.
+       inversion H1; subst; clear H1; simpl.
+       now apply RFlow.halts_next.
+    -- rewrite REnvironment.OP.P.add_neq_o in H1; auto.
+       now apply IH in H1.
+Qed.
+
+Lemma halts_puts t V :
+  halts t -> REnvironment.halts V -> halts (puts V t).
+Proof.
+  revert V. induction t using map_induction; intros.
+  - rewrite puts_Empty; auto; unfold halts; intros; inversion H2.
+  - rewrite puts_Add_spec; eauto. unfold Add in H0; rewrite H0 in *.
+    apply halts_add_spec_1 in H1 as [Hle Hlt1]; auto.
+    apply (IHt1 V) in Hlt1; auto. unfold puts_func.
+    destruct (V⌊x⌋ᵣᵦ) eqn:HfV; auto. destruct r; auto.
+    apply halts_add_spec; split; auto.
+    apply RFlow.halts_put; auto. apply H2 in HfV; now simpl in *. 
+Qed.
+
+
+
+
+(** *** Morphism *)
+
+#[global] 
+Instance in_rflow : 
+  Proper (Logic.eq ==> RFlows.eq ==> iff) In.
+Proof.
+  repeat red; intros; split; intros;
+  apply OP.P.Equal_Eqdom in H0; eapply OP.P.In_m in H0; eauto;
+  apply H0; eauto. 
+Qed.
+
+#[global] 
+Instance find_rflow : Proper (Logic.eq ==> RFlows.eq ==> Logic.eq) find.
+Proof. repeat red; intros; subst. now rewrite H0. Qed.
+
+#[global] 
+Instance Empty_rflow : Proper (RFlows.eq ==> iff) OP.P.Empty.
+Proof. red; red; intros; now apply Empty_eq_spec. Qed.
+
+#[export] 
+Instance Add_rflow : 
+Proper (Resource.eq ==> Logic.eq ==> RFlows.eq ==> RFlows.eq ==> iff) 
+            (@OP.P.Add RFlow.t).
+Proof. 
+  red; red; red; red; red; intros; subst; rewrite H. 
+  split; intros; unfold Add in *.
+  - rewrite <- H2; rewrite H0. now rewrite H1.
+  - rewrite H1. now rewrite H2.
+Qed.
+
+#[global] 
+Instance add_rflow : 
+Proper (Resource.eq ==> Logic.eq ==> RFlows.eq ==> RFlows.eq) 
+                                                          (@add RFlow.t).
+Proof.
+  repeat red; intros; subst; rewrite H1; now rewrite H.
+Qed. 
+
+#[global] 
+Instance Submap_env : 
+  Proper (RFlows.eq ==> RFlows.eq ==> iff) Submap.
+Proof. 
+  repeat red; intros; split; intros.
+  - rewrite Submap_eq_left_spec in H1; eauto.
+    rewrite Submap_eq_right_spec in H1; eauto.
+  - rewrite <- Submap_eq_left_spec in H1; eauto.
+    rewrite <- Submap_eq_right_spec in H1; eauto.
+Qed.
+
+End RFlows.
+
+(** *** Scope and Notations *)
+
+Declare Scope rflow_scope.
+Delimit Scope rflow_scope with rf.
+
+Definition 𝐅 := RFlows.t.
+
+Infix "⊆ᵣₔ" := RFlows.Submap (at level 20, no associativity). 
+Infix "∈ᵣₔ" := RFlows.Raw.In (at level 20, no associativity). 
+Notation "r '∉ᵣₔ' Re" := (~ (RFlows.Raw.In r Re)) (at level 20, 
+                                                                        no associativity). 
+Notation "∅ᵣₔ" := RFlows.Raw.empty (at level 20, no associativity). 
+Notation "'isEmptyᵣₔ(' Re ')'" := (RFlows.OP.P.Empty Re) (at level 20, no associativity). 
+Notation "'Addᵣₔ'" := (RFlows.OP.P.Add) (at level 20, no associativity). 
+Notation "'maxᵣₔ(' R ')'"  := (RFlows.Ext.max_key R) (at level 15).
+Notation "'newᵣₔ(' R ')'"  := (RFlows.Ext.new_key R) (at level 15).
+Notation "R '⌊' x '⌋ᵣₔ'"  := (RFlows.Raw.find x R) (at level 15, x constr).
+Notation "⌈ x ⤆ v '⌉ᵣₔ' R"  := (RFlows.Raw.add x v R) (at level 15, 
+                                                                          x constr, v constr).
+Notation "R ⌈ x ⩦ v '⌉ᵣₔ'"  := (RFlows.Raw.find x R = Some v) (at level 15, 
+                                                                                  x constr, 
+                                                                                  v constr).
+Notation "R ⌈ x ⩦ ⊥ '⌉ᵣₔ'"  := (RFlows.Raw.find x R = None) (at level 15, 
+                                                                                    x constr).
+
+Infix "=" := RFlows.eq : rflow_scope.
+
+#[global]
+Instance eq_equiv_re : Equivalence RFlows.eq.
+Proof. apply RFlows.OP.P.Equal_equiv. Qed.
+
+#[global] Instance max_re : Proper (RFlows.eq ==> Logic.eq) (RFlows.Ext.max_key).
+          Proof. apply RFlows.Ext.max_key_eq. Qed.
+
+#[global] Instance new_re : Proper (RFlows.eq ==> Logic.eq) (RFlows.Ext.new_key).
+          Proof. apply RFlows.Ext.new_key_eq. Qed.
+          
+#[global] 
+Instance in_rflow : 
+  Proper (Logic.eq ==> RFlows.eq ==> iff) (RFlows.Raw.In).
+Proof. apply RFlows.in_rflow. Qed.
+
+#[global] 
+Instance find_rflow : Proper (Logic.eq ==> RFlows.eq ==> Logic.eq) 
+                                                      (RFlows.Raw.find).
+Proof. apply RFlows.find_rflow. Qed.
+
+#[global] 
+Instance Empty_rflow : Proper (RFlows.eq ==> iff) (RFlows.OP.P.Empty).
+Proof. apply RFlows.Empty_rflow. Qed.
+
+#[global] 
+Instance Add_rflow : 
+Proper (Resource.eq ==> Logic.eq ==> RFlows.eq ==> RFlows.eq ==> iff) 
+                                                  (@RFlows.OP.P.Add RFlow.t).
+Proof. apply RFlows.Add_rflow. Qed. 
+
+#[global] 
+Instance add_rflow : 
+Proper (Resource.eq ==> Logic.eq ==> RFlows.eq ==> RFlows.eq) 
+                                                          (@RFlows.Raw.add RFlow.t).
+Proof. apply RFlows.add_rflow. Qed. 
+
+#[global] 
+Instance Submap_env : 
+  Proper (RFlows.eq ==> RFlows.eq ==> iff) RFlows.Submap.
+Proof. apply RFlows.Submap_env. Qed.
+
+#[global] 
+Instance Submap_env_po : PreOrder RFlows.Submap.
+Proof. apply RFlows.Submap_po. Qed. 
