theories/Syntax/RFlow.v
@@ -1,0 +1,62 @@
+From Coq Require Import Lists.Streams Structures.Equalities.
+From Mecha Require Import Term Evaluation Resource.
+From DeBrLevel Require Import LevelInterface.
+
+Module RFlow <: EqualityType.
+
+Import Streams.
+
+Definition t : Type := (Stream Λ * Stream Λ).
+
+Definition eq (t t' : t) := (EqSt (fst t) (fst t')) /\ (EqSt (snd t) (snd t')). 
+
+Definition next (rr : t) : Λ := 
+  let (inp,_) := rr in hd inp.
+
+Definition put (v : Λ) (rr : t) : t :=
+  let (inp,out) := rr in (tl inp,Cons v out).
+
+Definition put_opt (v : option Λ) (rr : t) : t :=
+  match v with
+    | Some v' => put v' rr
+    | _ => rr
+  end.
+
+Definition halts (rr : t) := 
+  ForAll (fun st => halts (Streams.hd st)) (fst rr) /\
+  ForAll (fun st => halts (Streams.hd st)) (snd rr).
+
+Lemma halts_next t : 
+  halts t -> Evaluation.halts (next t).
+Proof.
+  intros. destruct t; simpl; destruct H; simpl in *.
+  destruct s; simpl in *; inversion H; now simpl in *.
+Qed.
+
+Lemma halts_put t v :
+  halts t -> Evaluation.halts v -> halts (put v t).
+Proof.
+  intros; unfold put; destruct t; destruct H; split; simpl in *.
+  - inversion H; auto.
+  - split; simpl; auto.
+Qed. 
+
+Lemma halts_put_opt t v :
+  halts t -> match v with Some v => Evaluation.halts v | _ => True end -> halts (put_opt v t).
+Proof.
+  intros. destruct v; auto. unfold put_opt; now apply halts_put.
+Qed. 
+
+#[export]
+Instance eq_equiv : Equivalence eq.
+Proof.
+  split; unfold eq.
+  - red; intros; destruct x; simpl in *; split; apply EqSt_reflex.
+  - red; intros; destruct x,y; simpl in *; destruct H; split;
+    apply sym_EqSt; auto.
+  - red; intros; destruct x,y,z; simpl in *; destruct H,H0; split.
+    -- eapply trans_EqSt; eauto.
+    -- eapply trans_EqSt; eauto.
+Qed.
+
+End RFlow.
